finished proof of the sample

Mt/sample.lean
@@ -32,12 +32,19 @@ def spec : Mt.Spec :={
   validate := fun ⟨luft, min_x⟩ ⟨x, y⟩ => x ≥ y + luft ∧ x ≥ min_x
   reservations_can_be_dropped :=by
     simp only []
-    intro r r' state h
-    constructor
-    . exact calc
-        state.y + r.luft ≤ state.y + (r.luft + r'.luft) :=by simp_arith
-        _                ≤ state.x                      :=h.left
-    . sorry -- TODO
+    intro ⟨env_luft, (env_min_x : Nat)⟩ ⟨luft, (min_x : Nat)⟩ ⟨x, y⟩
+      (h : x ≥ y + (env_luft + luft) ∧ x ≥ Nat.max env_min_x min_x)
+
+    show x ≥ y + env_luft ∧ x ≥ env_min_x
+
+    cases h ; constructor
+    . show x ≥ y + env_luft
+      exact calc
+        y + env_luft ≤ y + (env_luft + luft) :=by simp_arith
+                   _ ≤ x                     :=by assumption
+    . show x ≥ env_min_x
+      rename x ≥ Nat.max env_min_x min_x => h
+      exact (nat_max_le.mp h).left 
 }
 
 open Mt
@@ -98,19 +105,62 @@ theorem thread1_valid : thread1.valid_for_reservation' ReservationInstance.empty
     . show x ≥ y + 1 + env_luft
       rw [Nat.add_right_comm] ; assumption
   
-  --clear luft min_x luft_def
+  clear luft min_x luft_def
   intro ⟨luft, min_x⟩ ⟨⟩ ⟨⟩
   apply valid_for_reservation_bind (spec :=spec) _ _ _ λ ⟨_, min_x⟩ y => min_x = y
   . -- validate `let py = y` with `min_x := py`
     -------------------------------------------
     apply valid_for_reservation_read
-    intro ⟨x, y⟩ ⟨env_luft, env_min_x⟩ initial_valid
+    intro ⟨x, y⟩ ⟨env_luft, (env_min_x : Nat)⟩ initial_valid
     simp only [and_true]
 
     have : x ≥ y + (env_luft + luft) ∧ x ≥ Nat.max env_min_x min_x :=initial_valid
-
     show x ≥ y + env_luft ∧ x ≥ Nat.max env_min_x y
+
     cases this ; constructor
-    . sorry
-    . sorry
-  sorry
+    . show y + env_luft ≤ x
+      exact calc
+        y + env_luft ≤ y + (env_luft + luft) :=by simp_arith
+                   _ ≤ x                     :=by assumption
+    . show Nat.max env_min_x y ≤ x
+      apply nat_max_le.mpr ; constructor
+      . show env_min_x ≤ x
+        rename x ≥ Nat.max env_min_x min_x => h
+        exact (nat_max_le.mp h).left
+      . show y ≤ x
+        exact calc
+          y ≤ y + (env_luft + luft) :=by simp_arith
+          _ ≤ x                     :=by assumption
+
+  clear luft min_x
+  intro ⟨luft, min_x⟩ (py : Nat) min_x_def
+  apply valid_for_reservation_bind (spec :=spec) _ _ _ λ _ x => x ≥ py
+  . -- validate `let px = x` knowing min_x = py
+    -------------------------------------------
+    have min_x_def : min_x = py :=min_x_def
+    apply valid_for_reservation_read
+    intro ⟨x, y⟩ ⟨env_luft, (env_min_x : Nat)⟩ initial_valid
+
+    have : x ≥ y + (env_luft + luft) ∧ x ≥ Nat.max env_min_x min_x :=initial_valid
+    show (x ≥ y + env_luft ∧ x ≥ Nat.max env_min_x 0) ∧ x ≥ py
+    
+    cases this ; constructor ; constructor
+    . show y + env_luft ≤ x
+      calc
+        y + env_luft ≤ y + (env_luft + luft) :=by simp_arith
+                   _ ≤ x                     :=by assumption
+    . show x ≥ Nat.max env_min_x 0
+      rw [nat_max_zero]
+      rename x ≥ Nat.max env_min_x min_x => h
+      exact (nat_max_le.mp h).left
+    . show x ≥ py
+      suffices x ≥ min_x by rw [<- min_x_def] ; assumption
+      rename x ≥ Nat.max env_min_x min_x => h
+      exact (nat_max_le.mp h).right
+  
+  clear luft min_x min_x_def
+  intro ⟨luft, min_x⟩ (px : Nat) px_gt_py
+
+  have : px ≥ py :=px_gt_py -- for the assertion
+
+  exact valid_for_reservation_pure (spec :=spec) _ _ (λ _ _ => True) ⟨⟩
